Strata/DL/Util/Maps.lean
@@ -24,6 +24,21 @@ def Maps.format' [ToFormat (Map α β)] (ms : Maps α β) : Format :=
 instance[ToFormat (Map α β)] : ToFormat (Maps α β) where
   format := Maps.format'
 
+def Maps.keys (ms : Maps α β) : List α :=
+  match ms with
+  | [] => []
+  | m :: mrest => m.keys ++ Maps.keys mrest
+
+def Maps.values (ms : Maps α β) : List β :=
+  match ms with
+  | [] => []
+  | m :: mrest => m.values ++ Maps.values mrest
+
+def Maps.isEmpty (m : Maps α β) : Bool :=
+  match m with
+  | [] => true
+  | _ => false
+
 /--
 Add Map `m` to the beginning of Maps `ms`.
 -/
@@ -97,6 +112,20 @@ def Maps.findD [DecidableEq α] (ms : Maps α β) (x : α) (d : β) : β :=
     | some v => v
 
 /--
+Remove the first occurence of element with key `a'` in `m`, starting from the
+newest map.
+-/
+def Maps.remove [DecidableEq α] [BEq (Map α β)] (m : Maps α β) (a' : α) : Maps α β :=
+  match m with
+  | [] => []
+  | m :: mrest =>
+    let m' := Map.remove m a'
+    if m' == m then
+      m :: (remove mrest a')
+    else
+      m' :: (remove mrest a')
+
+/--
 Erase `x` and its associated value from `ms`.
 -/
 def Maps.erase [DecidableEq α] (ms : Maps α β) (x : α) : Maps α β :=
@@ -159,5 +188,154 @@ def Maps.addInOldest [DecidableEq α] (ms : Maps α β) (xs : List α) (vs : Lis
   | x :: xrest, v :: vrest =>
     let ms := Maps.insertInOldest ms x v
     Maps.addInOldest ms xrest vrest
+
+---------------------------------------------------------------------
+
+theorem Maps.find?_mem_keys [DecidableEq α] (m : Maps α β)
+  (h : Maps.find? m k = some v) :
+  k ∈ Maps.keys m := by
+  induction m with
+  | nil => simp_all [Maps.find?]
+  | cons head tail ih =>
+    simp [Maps.find?] at h
+    split at h
+    · simp [Maps.keys]; simp_all
+    · rename_i _ v1 heq
+      simp at h; subst v1
+      simp [Maps.keys]
+      have := @Map.find?_mem_keys α β k v _ head heq
+      simp_all
+  done
+
+theorem Maps.find?_mem_values [DecidableEq α] (m : Maps α β)
+  (h : Maps.find? m k = some v) :
+  v ∈ Maps.values m := by
+  induction m with
+  | nil => simp [Maps.find?] at h
+  | cons head tail ih =>
+    simp [Maps.find?] at h
+    split at h
+    · simp [Maps.values]; simp_all
+    · rename_i _ v1 heq
+      simp at h; subst v1
+      simp [Maps.values]
+      have := @Map.find?_mem_values α β k v _ head heq
+      simp_all
+
+theorem Maps.find?_of_not_mem_values [DecidableEq α] (S : Maps α β)
+  (h1 : Maps.find? S i = none) : i ∉ Maps.keys S := by
+  induction S; all_goals simp_all [Maps.keys]
+  rename_i _ head tail ih
+  simp [Maps.find?] at h1
+  split at h1 <;> simp_all
+  rename_i h
+  exact Map.find?_of_not_mem_values head h
+  done
+
+private theorem Maps.insert_fresh_key_subset [DecidableEq α] (ms : Maps α β)
+  (h : Maps.find? ms key = none) :
+  (Maps.insert ms key val).keys ⊆ key :: Maps.keys ms := by
+  simp_all [Maps.insert, Maps.pop, Maps.push, Maps.newest, Maps.keys]
+  split <;> simp_all [Map.insert, Maps.keys, Map.keys]
+  rename_i ms m ms_rest
+  have := @Map.insert_keys _ _ key val _ m
+  grind
+  done
+
+private theorem Maps.insert_fresh_key_subset_value [DecidableEq α] (ms : Maps α β)
+  (h : Maps.find? ms key = none) :
+  (Maps.insert ms key val).values ⊆ val :: Maps.values ms := by
+  simp_all [Maps.insert, Maps.pop, Maps.push, Maps.newest, Maps.values]
+  split <;> simp_all [Map.insert, Maps.values, Map.values]
+  rename_i ms m ms_rest
+  have := @Map.insert_values _ _ key val _ m
+  grind
+  done
+
+private theorem Maps.insert_key_update_subset [DecidableEq α] (ms : Maps α β)
+  (h : ¬ Maps.find? ms key = none) :
+  (Maps.insert ms key val).keys ⊆ Maps.keys ms := by
+  simp_all [Maps.insert, Maps.pop, Maps.push, Maps.newest]
+  split <;> simp_all
+  rename_i v heq
+  induction ms
+  case nil => simp_all [Maps.find?]
+  case cons hd tl ih =>
+    simp_all [Maps.update, Maps.find?]
+    split <;> simp_all [Maps.keys]
+    rename_i heq_hd_key
+    have := @Map.find?_mem_keys _ _ key v _ hd heq_hd_key
+    have := @Map.insert_keys _ _ key val _ hd
+    grind
+  done
+
+private theorem Maps.insert_key_update_subset_value [DecidableEq α] (ms : Maps α β)
+  (h : ¬ Maps.find? ms key = none) :
+  (Maps.insert ms key val).values ⊆ val :: Maps.values ms := by
+  simp_all [Maps.insert, Maps.pop, Maps.push, Maps.newest]
+  split <;> simp_all
+  rename_i v heq
+  induction ms
+  case nil => simp_all [Maps.find?]
+  case cons hd tl ih =>
+    simp_all [Maps.update, Maps.find?]
+    split <;> simp_all [Maps.values]
+    rename_i heq_hd_key
+    · have := @Map.find?_mem_values _ _ key val _ hd;
+      have := @Map.insert_values _ _ key val _ hd;
+      grind
+    · have := @Map.find?_mem_values _ _ key val _ hd
+      have := @Map.insert_values _ _ key val _ hd
+      grind
+  done
+
+theorem Maps.insert_keys_subset [DecidableEq α] (ms : Maps α β) :
+  (Maps.insert ms key val).keys ⊆ key :: Maps.keys ms := by
+  have h1 := @Maps.insert_fresh_key_subset _ _ key val _ ms
+  have h2 := @Maps.insert_key_update_subset _ _ key val _ ms
+  grind
+  done
+
+theorem Maps.insert_values_subset [DecidableEq α] (ms : Maps α β) :
+  (Maps.insert ms key val).values ⊆ val :: Maps.values ms := by
+  have h1 := @Maps.insert_fresh_key_subset_value _ _ key val _ ms
+  have h2 := @Maps.insert_key_update_subset_value _ _ key val _ ms
+  grind
+
+@[simp]
+theorem Maps.keys_of_push_empty :
+  (Maps.push ms []).keys = ms.keys := by
+  simp_all [Maps.push, Maps.keys, Map.keys]
+
+@[simp]
+theorem Maps.values_of_push_empty :
+  (Maps.push ms []).values = ms.values := by
+  simp_all [Maps.push, Maps.values, Map.values]
+
+theorem Maps.mem_keys_of_mem_keys_remove [DecidableEq α] [BEq (Map α β)]
+  (ms : Maps α β) (k1 k2 : α) (h : k2 ∈ (Maps.remove ms k1).keys) :
+  k2 ∈ ms.keys := by
+  induction ms
+  case nil => simp_all [Maps.keys, Maps.remove]
+  case cons m ms ih =>
+    simp_all [Maps.remove, Maps.keys]
+    split at h <;> simp_all [Maps.keys]
+    · grind
+    · cases h
+      · simp [@Map.mem_keys_of_mem_keys_remove _ _ _ m k1 k2 (by assumption)]
+      · simp_all
+
+theorem Maps.mem_values_of_mem_keys_remove [DecidableEq α] [BEq (Map α β)]
+  (ms : Maps α β) (k : α) (v : β) (h : v ∈ (Maps.remove ms k).values) :
+  v ∈ ms.values := by
+  induction ms
+  case nil => simp_all [Maps.values, Maps.remove]
+  case cons m ms ih =>
+    simp_all [Maps.remove, Maps.values]
+    split at h <;> simp_all [Maps.values]
+    · grind
+    · cases h
+      · simp [@Map.mem_values_of_mem_keys_remove _ _ _ m k v (by assumption)]
+      · simp_all
 
 ---------------------------------------------------------------------
